\section{Loop filter}
\subsection{Passive Lag-lead Filter}
\begin{equation*}
    F(s) = \dfrac{1+s\tau_2}{1+s(\tau_1 + \tau_2)}
\end{equation*}
\begin{align*}
    \Rightarrow H(s) &= \dfrac{K_{pd}\cdot K_{vco}\cdot \dfrac{1+s\tau_2}{1+s(\tau_1 + \tau_2)}}{K_{pd}\cdot K_{vco}\cdot \dfrac{1+s\tau_2}{1+s\left(\tau_1 + \tau_2\right)}+N\cdot s}\\
    &= \dfrac{\dfrac{K_{pd}\cdot K_{vco}\cdot \tau_2}{N\cdot \left(\tau_1 + \tau_2\right)}\cdot \left(s+\dfrac{1}{\tau_2}\right)}{s^2 + \dfrac{1+\dfrac{K_{pd}\cdot K_{vco}\cdot \tau_2}{N}}{\tau_1 + \tau_2}\cdot s + \dfrac{K_{pd}\cdot K_{vco}}{N\cdot \left(\tau_1 + \tau_2\right)}} 
\end{align*}
\begin{align*}
    \Rightarrow 2\omega_n \zeta &= \dfrac{1+K_{pd}\cdot K_{vco}\cdot \tau_2}{\tau_1 +\tau_2} &\omega_n^2 &= \dfrac{K_{pd} \cdot K_{vco}}{N\cdot \left(\tau_1 + \tau_2\right)}\\
    \Rightarrow \omega_n &= \sqrt{\dfrac{K_{pd}\cdot K_{vco}}{N\cdot \left(\tau_1 + \tau_2 \right)}} &\zeta &= \dfrac{N+K_{pd}\cdot K_{vco}\cdot \tau_2}{N\cdot \left(\tau_1 + \tau_2\right) \cdot 2\omega_n} = \dfrac{\omega_n}{2}\cdot \left(\tau_2 + \dfrac{N}{K_{pd}\cdot K_{vco}}\right)
\end{align*}
